@base <http://vocab.ub.uni-leipzig.de/bibrm/> . 
@prefix bibrm:  <http://vocab.ub.uni-leipzig.de/bibrm/> .
@prefix cc:     <http://creativecommons.org/ns#> .
@prefix dc:     <http://purl.org/dc/elements/1.1/> .
@prefix dct:    <http://purl.org/dc/terms/> .
@prefix doap:   <http://usefulinc.com/ns/doap#>.
@prefix foaf:   <http://xmlns.com/foaf/0.1/> .
@prefix owl:    <http://www.w3.org/2002/07/owl#> .
@prefix rdf:    <http://www.w3.org/1999/02/22-rdf-syntax-ns#> .
@prefix rdfs:   <http://www.w3.org/2000/01/rdf-schema#> .
@prefix skos:   <http://www.w3.org/2004/02/skos/core#> .
@prefix vann:   <http://purl.org/vocab/vann/>.
@prefix xsd:    <http://www.w3.org/2001/XMLSchema#> .

<> a owl:Ontology;
  foaf:maker <http://aksw.org/NormanRadtke>, <http://aksw.org/AndreasNareike>, <http://aksw.org/NatanaelArndt> ;
  doap:maintainer <http://aksw.org/NormanRadtke>;
  doap:homepage <http://aksw.org/Projects/ERM>;
  cc:attributionName "AKSW & Universitätsbibliothek Leipzig" ;
  vann:changes <https://github.com/ERM-HD/vocab.bibrm/commits/master/bibrm.ttl>;
  vann:preferredNamespacePrefix "bibrm";
  vann:preferredNamespaceUri "http://vocab.ub.uni-leipzig.de/bibrm/";
  rdfs:label "Vocabulary for Library Electronic Resource Management";
  rdfs:isDefinedBy <> .

#################################
############ Classes ############
#################################

bibrm:LicenseContract rdf:type        owl:Class ;
                    rdfs:comment    "A class modeling a business contract between two or more parties"@en ;
                    rdfs:isDefinedBy <> ;
                    rdfs:subClassOf bibrm:BibliographicResource ,
                                    [ rdf:type owl:Restriction ;
                                    owl:onProperty bibrm:licensedBy ;
                                    owl:minCardinality "1"^^xsd:nonNegativeInteger
                                    ] ,
                                    [ rdf:type owl:Restriction ;
                                    owl:onProperty bibrm:licensedTo ;
                                    owl:minCardinality "1"^^xsd:nonNegativeInteger
                                    ] ,
                                    [ rdf:type owl:Restriction ;
                                    owl:onProperty bibrm:hasItem ;
                                    owl:minCardinality "0"^^xsd:nonNegativeInteger ;
                                    ] ,
                                    [ rdf:type owl:Restriction ;
                                    owl:onProperty bibrm:price ;
                                    owl:minCardinality "0"^^xsd:nonNegativeInteger ;
                                    owl:maxCardinality "1"^^xsd:nonNegativeInteger
                                    ] ,
                                    [ rdf:type owl:Restriction ;
                                    owl:onProperty bibrm:licenseStartDate ;
                                    owl:minCardinality "0"^^xsd:nonNegativeInteger ;
                                    owl:maxCardinality "1"^^xsd:nonNegativeInteger
                                    ] ,
                                    [ rdf:type owl:Restriction ;
                            owl:onProperty bibrm:licenseEndDate ;
                            owl:minCardinality "0"^^xsd:nonNegativeInteger ;
                            owl:maxCardinality "1"^^xsd:nonNegativeInteger
                            ] .

bibrm:BibliographicResource rdf:type owl:Class ;
            rdfs:label      "Bibliographic Item"@en; 
            rdfs:comment    "A class containing all items a bibliotheca shares offers it's customers"@en ;
            rdfs:comment    "Ein BibItem ist ein Ding, welches die Bibliothek ihren Nutzern zur Nutzung anbietet"@de ;
            rdfs:isDefinedBy <> ;
            rdfs:subClassOf [ rdf:type owl:Restriction ;
                            owl:onProperty dc:publisher ;
                            owl:minCardinality "1"^^xsd:nonNegativeInteger
                            ] ,
                            [ rdf:type owl:Restriction ;
                            owl:onProperty dc:title ;
                            owl:cardinality "1"^^xsd:nonNegativeInteger
                            ] .


bibrm:Organization    rdf:type        owl:Class ;
            rdfs:label      "Body"@en ;
            rdfs:comment    "A class containing entities like publishers or license agents"@en ;
            rdfs:comment    "Diese Klasse beinhaltet Institutionen wie Verlage oder Unternehmen für den Vertrieb bzw. die Lizensierung von bibrm:BibItems"@de ;
            rdfs:isDefinedBy <> ;
            rdfs:subClassOf dct:Agent .

bibrm:Contact rdf:type        owl:Class ;
            rdfs:label      "Contact"@en ;
            rdfs:isDefinedBy <> ;
            rdfs:subClassOf foaf:Person ,
                            [ rdf:type owl:Restriction ;
                            owl:onProperty foaf:name ;
                            owl:cardinality "1"^^xsd:nonNegativeInteger
                            ] .

bibrm:Contract    rdf:type        owl:Class ;
                rdfs:label      "Contract"@en ;
                rdfs:label      "Vertrag"@de ;
                rdfs:isDefinedBy <> ;
                rdfs:comment    ""@en ;
                rdfs:comment    ""@de .

bibrm:ContractItem    rdf:type        owl:Class ;
                    rdfs:label      "Contract item"@en ;
                    rdfs:comment    "The object/thing of a contract"@en ;
                    rdfs:comment    "Der Gegenstand eines Vertrags"@de ;
                    rdfs:isDefinedBy <> ;
                    rdfs:subClassOf [ rdf:type owl:Restriction ;
                                    owl:onProperty bibrm:hasItem ;
                                    owl:minCardinality "1"^^xsd:nonNegativeInteger
                                    ] .

bibrm:EJournal    rdf:type        owl:Class ;
                rdfs:label      "E-Journal"@en ;
                rdfs:comment    "An electronic journal"@en ;
                rdfs:comment    "Eine elektronische Zeitschrift"@de ;
                rdfs:isDefinedBy <> ;
                rdfs:subClassOf bibrm:Journal ,
                                [ rdf:type owl:Restriction ;
                                owl:onProperty bibrm:hasEISSN ;
                                owl:minCardinality "1"^^xsd:nonNegativeInteger
                                ] ,
                                [ rdf:type owl:Restriction ;
                                owl:onProperty bibrm:hasPISSN ;
                                owl:cardinality "0"^^xsd:nonNegativeInteger
                                ] .

bibrm:Journal rdf:type        owl:Class ;
            rdfs:label      "Journal"@en ;
            rdfs:comment    "A Journal. This class can be used if a unique reference to either the electronic or printed version of a journal is not given"@en ;
            rdfs:comment    "Eine Zeitschrift, zu welcher die eindeutige Refferenz auf die elektronische oder gedruckte Ausgabe nicht gegeben ist."@de ;
            rdfs:isDefinedBy <> ;
            rdfs:subClassOf bibrm:BibItem ,
                            [ rdf:type owl:Restriction ;
                            owl:onProperty bibrm:hasPISSN ;
                            owl:cardinality "0"^^xsd:nonNegativeInteger
                            ] ,
                            [ rdf:type owl:Restriction ;
                            owl:onProperty bibrm:hasEISSN ;
                            owl:cardinality "0"^^xsd:nonNegativeInteger
                            ] ,
                            [ rdf:type owl:Restriction ;
                            owl:onProperty bibrm:title ;
                            owl:minCardinality "0"^^xsd:nonNegativeInteger
                            ] .

bibrm:LicencePackage  rdf:type        owl:Class ;
                    rdfs:label      "Licence Package"@en ;
                    rdfs:comment    "A package licenced in a licence contract containing items (e.g. journals, books) a bibliotheca offers it's customers"@en ;
                    rdfs:comment    "Ein Lizenzpaket bestehend aus Subjekten wie Büchern oder Zeitschriften, welche eine Bibliothek ihren Nutzern anbietet"@de ;
                    rdfs:isDefinedBy <> ;
                    rdfs:subClassOf bibrm:ContractItem .

bibrm:PJournal    rdf:type        owl:Class ;
                rdfs:label      "Printed Journal"@en ;
                rdfs:comment    "A printed journal"@en ;
                rdfs:comment    "Eine gedruckte Zeitschrift"@de ;
                rdfs:isDefinedBy <> ;
                rdfs:subClassOf bibrm:Journal ,
                                [ rdf:type owl:Restriction ;
                                owl:onProperty bibrm:hasPISSN ;
                                owl:minCardinality "1"^^xsd:nonNegativeInteger
                                ] ,
                                [ rdf:type owl:Restriction ;
                                owl:onProperty bibrm:hasEISSN ;
                                owl:cardinality "0"^^xsd:nonNegativeInteger
                                ] .

########################################
########### ObjectProperties ###########
########################################


bibrm:hasItem rdf:type    owl:ObjectProperty, rdf:Property ;
            rdfs:label  "has item"@en ;
            rdfs:isDefinedBy <> ;
            rdfs:domain bibrm:LicenceContract ;
            rdfs:range  bibrm:ContractItem .

bibrm:hasPISSN    rdf:type    owl:ObjectProperty, rdf:Property ;
                rdfs:label  "has P-ISSN"@en ;
                rdfs:isDefinedBy <> ;
                rdfs:domain bibrm:Journal .

bibrm:hasEISSN    rdf:type    owl:ObjectProperty, rdf:Property ;
                rdfs:label  "has E-ISSN"@en ;
                rdfs:isDefinedBy <> ;
                rdfs:domain bibrm:Journal .
bibrm:licensedBy   rdf:type        owl:ObjectProperty, rdf:Property ;
                rdfs:label      "offered by"@en ;
                rdfs:comment    "The partie of the contract offering the lawfull object"@en ;
                rdfs:isDefinedBy <> ;
                rdfs:domain     bibrm:Contract ;
                rdfs:range      bibrm:Body .

bibrm:licensedTo   rdf:type        owl:ObjectProperty, rdf:Property ;
                rdfs:label      "offered to"@en ;
                rdfs:comment    "The partie of the contract receiving the lawfull object"@en ;
                rdfs:isDefinedBy <> ;
                rdfs:domain     bibrm:Contract .

#################################
########### Datatypes ###########
#################################

bibrm:licenseEndDate    rdf:type    owl:DatatypeProperty, rdf:Property ;
               rdfs:label  "end date"@en ;
               rdfs:label  "Enddatum"@de ;
               rdfs:isDefinedBy <> ;
               rdfs:domain bibrm:Contract ;
               rdfs:range  xsd:date .

bibrm:field      rdf:type     owl:DatatypeProperty, rdf:Property ;
               rdfs:label   "field"@en ;
               rdfs:label   "Fachgebiet"@de ;
               rdfs:comment "The field predicate can be used to classify bibliographic items"@en ;
               rdfs:comment "Das Prädikat ermgölicht die Angabe von Fachgebieten"@de ;
               rdfs:isDefinedBy <> ;
               rdfs:domain  bibrm:BibItem .

bibrm:name   rdf:type            owl:DatatypeProperty, rdf:Property ;
           rdfs:isDefinedBy <> ;
           rdfs:subPropertyOf  foaf:name .

bibrm:price   rdf:type    owl:DatatypeProperty, rdf:Property ;
            rdfs:label  "price"@en ;
            rdfs:label  "Preis"@de ;
            rdfs:comment    "The price a item costs the biblitheca to offer that item to their users"@en ;
            rdfs:comment    "Der Anschaffungs-/Nutzungspreis, den die Bibliothek für ein BibItem bezahlt"@de ;
            rdfs:isDefinedBy <> ;
            rdfs:domain bibrm:BibItem ;
            rdfs:range  xsd:double .

bibrm:publisher  rdf:type            owl:DatatypeProperty, rdf:Property ;
               rdfs:isDefinedBy <> ;
               rdfs:subPropertyOf  dc:publisher .

bibrm:licenseStartDate   rdf:type    owl:DatatypeProperty, rdf:Property ;
                rdfs:label  "start date"@en ;
                rdfs:label  "Startdatum"@de ;
                rdfs:isDefinedBy <> ;
                rdfs:domain bibrm:Contract ;
                rdfs:range  xsd:date .
