@base <http://vocab.ub.uni-leipzig.de/bibrm/> . 
@prefix bibrm:  <http://vocab.ub.uni-leipzig.de/bibrm/> .
@prefix bibo:   <http://purl.org/ontology/bibo/> .
@prefix cc:     <http://creativecommons.org/ns#> .
@prefix dc:     <http://purl.org/dc/elements/1.1/> .
@prefix dct:    <http://purl.org/dc/terms/> .
@prefix doap:   <http://usefulinc.com/ns/doap#>.
@prefix foaf:   <http://xmlns.com/foaf/0.1/> .
@prefix owl:    <http://www.w3.org/2002/07/owl#> .
@prefix rdf:    <http://www.w3.org/1999/02/22-rdf-syntax-ns#> .
@prefix rdfs:   <http://www.w3.org/2000/01/rdf-schema#> .
@prefix skos:   <http://www.w3.org/2004/02/skos/core#> .
@prefix vann:   <http://purl.org/vocab/vann/>.
@prefix xsd:    <http://www.w3.org/2001/XMLSchema#> .

<> a owl:Ontology;
  foaf:maker <http://aksw.org/NormanRadtke>, <http://aksw.org/AndreasNareike>, <http://aksw.org/NatanaelArndt>, <http://aksw.org/ThomasRiechert>, <http://aksw.org/Partner/LydiaUnterdoerfel>, <http://aksw.org/Partner/BjoernMuschall>, <http://aksw.org/Partner/LeanderSeige> ;
  doap:maintainer <http://aksw.org/NormanRadtke>;
  doap:homepage <http://aksw.org/Projects/ERM>;
  cc:attributionName "AKSW & Universitätsbibliothek Leipzig" ;
  vann:changes <https://github.com/ERM-HD/vocab.bibrm/commits/master/bibrm.ttl>;
  vann:preferredNamespacePrefix "bibrm";
  vann:preferredNamespaceUri "http://vocab.ub.uni-leipzig.de/bibrm/";
  rdfs:label "Vocabulary for Library Electronic Resource Management";
  rdfs:isDefinedBy <> .

#################################
############ Classes ############
#################################

bibrm:LicenseContract rdf:type        owl:Class ;
                      rdfs:label      "LicenseContract"@en ;
                      rdfs:label      "Lizenzvertrag"@de ;
                      rdfs:comment    "A class modeling a business contract between the library and one or more parties. Item of the contract are licenses."@en ;
                      rdfs:comment    "Ein Geschäftsvertrag zwischen der Bibliothek und weiteren Partnern. Gegenstand des Vertrags sind Lizenzen."@de ;
                      rdfs:isDefinedBy <> ;
                      rdfs:subClassOf bibrm:ContractItem ,
                                      dct:LicenseDocument ,
                                      [ rdf:type owl:Restriction ;
                                      owl:onProperty bibrm:licensee ;
                                      owl:minCardinality "1"^^xsd:nonNegativeInteger
                                      ] ,
                                      [ rdf:type owl:Restriction ;
                                      owl:onProperty bibrm:licensor ;
                                      owl:minCardinality "1"^^xsd:nonNegativeInteger
                                      ] ,
                                      [ rdf:type owl:Restriction ;
                                      owl:onProperty bibrm:hasItem ;
                                      owl:minCardinality "0"^^xsd:nonNegativeInteger ;
                                      ] ,
                                      [ rdf:type owl:Restriction ;
                                      owl:onProperty bibrm:price ;
                                      owl:minCardinality "0"^^xsd:nonNegativeInteger ;
                                      owl:maxCardinality "1"^^xsd:nonNegativeInteger
                                      ] ,
                                      [ rdf:type owl:Restriction ;
                                      owl:onProperty bibrm:licenseStartDate ;
                                      owl:cardinality "1"^^xsd:nonNegativeInteger
                                      ] ,
                                      [ rdf:type owl:Restriction ;
                                      owl:onProperty bibrm:licenseEndDate ;
                                      owl:cardinality "1"^^xsd:nonNegativeInteger
                                      ] .

bibrm:BibliographicResource rdf:type owl:Class ;
                            rdfs:label      "Bibliographic Item"@en;
                            rdfs:label      "Bibliographische Ressource"@de ;
                            rdfs:comment    "A class containing all items a library offers it's users."@en ;
                            rdfs:comment    "Bibliographische Ressourcen sind alle Dinge, welche die Bibliothek ihren Nutzern anbietet."@de ;
                            rdfs:isDefinedBy <> ;
                            rdfs:subClassOf [ rdf:type owl:Restriction ;
                                            owl:onProperty dc:publisher ;
                                            owl:minCardinality "0"^^xsd:nonNegativeInteger
                                            ] ,
                                            [ rdf:type owl:Restriction ;
                                            owl:onProperty dc:title ;
                                            owl:cardinality "1"^^xsd:nonNegativeInteger
                                            ] .


bibrm:Organization rdf:type owl:Class ;
                   rdfs:subClassOf foaf:Organization ;
                   rdfs:label      "Organization"@en ;
                   rdfs:label      "Organisation"@de ;
                   rdfs:comment    "A class containing entities like publishers or license agents"@en ;
                   rdfs:comment    "Diese Klasse beinhaltet Institutionen wie Verlage oder Unternehmen für den Vertrieb bzw. die Lizenzierung von bibrm:BibliographicResources"@de ;
                   rdfs:isDefinedBy <> .

#TODO should become a subclass of contacts defined by schema.org
bibrm:Contact rdf:type        owl:Class ;
              rdfs:label      "Contact"@en ;
              rdfs:label      "Kontakt"@de ;
              rdfs:comment    "A class containing name, adress, phone number, organization and other contact information about a person "@en ;
              rdfs:comment    "Diese Klasse beinhaltet Kontaktinformationen einer Person, z.B. Name, Adresse, Organisation usw."@de ;
              rdfs:isDefinedBy <> ;
              rdfs:subClassOf foaf:Person ,
                              [ rdf:type owl:Restriction ;
                              owl:onProperty foaf:name ;
                              owl:cardinality "1"^^xsd:nonNegativeInteger
                              ] .

# TODO Think over if neccessary
bibrm:ContractItem  rdf:type        owl:Class ;
                    rdfs:label      "Contract item"@en ;
                    rdfs:label      "Vertragsgegenstand"@de ;
                    rdfs:comment    "The object/thing of a contract"@en ;
                    rdfs:comment    "Der Gegenstand eines Vertrags"@de ;
                    rdfs:isDefinedBy <> .

bibrm:Journal rdf:type        owl:Class ;
              rdfs:label      "Journal"@en ;
              rdfs:label      "Zeitschrift"@en ;
              rdfs:comment    "A Journal. This class can be used if a unique reference to either the electronic or printed version of a journal is not given"@en ;
              rdfs:comment    "Eine Zeitschrift, zu welcher die eindeutige Refferenz auf die elektronische oder gedruckte Ausgabe nicht gegeben ist."@de ;
              rdfs:isDefinedBy <> ;
              rdfs:subClassOf bibrm:BibliographicResource ,
                              bibo:Journal ,
                              [ rdf:type owl:Restriction ;
                              owl:onProperty bibrm:hasPISSN ;
                              owl:minCardinality "0"^^xsd:nonNegativeInteger
                              ] ,
                              [ rdf:type owl:Restriction ;
                              owl:onProperty bibrm:hasEISSN ;
                              owl:minCardinality "0"^^xsd:nonNegativeInteger
                              ] .

bibrm:Publisher rdf:type        owl:Class ;
                rdfs:label      "Publisher"@en ;
                rdfs:label      "Verlag"@de ;
                rdfs:comment    "A Class for containing organizations in a role of a publisher "@en ;
                rdfs:comment    "Eine Klasse für Organisation, die als Verlag auftreten."@de ;
                rdfs:isDefinedBy <> ;
                rdfs:subClassOf  bibrm:Organization .

bibrm:LicensingAgent rdf:type        owl:Class ;
                     rdfs:label      "Licensing Agent"@en ;
                     rdfs:label      "Lieferant"@de ;
                     rdfs:comment    "A Class for containing organizations in a role of a licensing agent "@en ;
                     rdfs:comment    "Diese Klasse modelliert Organisationen, die als Zahlungsempfänger/Zwischenhändler auftreten"@de ;
                     rdfs:isDefinedBy <> ;
                     rdfs:subClassOf  bibrm:Organization .

bibrm:Library   rdf:type        owl:Class ;
                rdfs:label      "Library"@en ;
                rdfs:label      "Bibliothek"@de ;
                rdfs:comment    "A class modeling organizations in the role of a library"@en ;
                rdfs:comment    "Ein Modell für Organisationen in der Rolle einer Bibliothek"@de ;
                rdfs:isDefinedBy <> ;
                rdfs:subClassOf  bibrm:Organization .

bibrm:Consortium rdf:type       owl:Class ;
                 rdfs:label      "Consortium"@en ;
                 rdfs:label      "Konsortium"@de ;
                 rdfs:comment    "A Class for containing organizations in the role of a consortium, a cooporation of libraries."@en ;
                 rdfs:comment    "Diese Klasse modelliert Organisationen, die als Konsortium, einem Zusammenschluss von Bibliotheken, auftreten"@de ;
                 rdfs:isDefinedBy <> ;
                 rdfs:subClassOf  bibrm:Organization .

bibrm:Interface rdf:type        owl:Class ;
                rdfs:label      "Interface"@en ;
                rdfs:label      "Schnittstelle"@de ;
                rdfs:comment    "A Class for interfaces that can be used to get information about journals or to read the journals "@en ;
                rdfs:comment    "Eine Klasse für Schittstellen um elektronische Medien oder Informationen zu solchen zu lesen"@de ;
                rdfs:isDefinedBy <> .

bibrm:LicensePackage rdf:type        owl:Class ;
                     rdfs:label      "License Package"@en ;
                     rdfs:label      "Paket"@de ;
                     rdfs:comment    "A package containing items (e.g. e-journals, e-books) a library offers it's customers"@en ;
                     rdfs:comment    "Ein Paket beinhaltet elektronische Bücher oder Zeitschriften, welche eine Bibliothek ihren Nutzern anbietet"@de ;
                     rdfs:isDefinedBy <> ;
                     rdfs:subClassOf bibrm:ContractItem ,
                                     [ rdf:type owl:Restriction ;
                                     owl:onProperty bibrm:hasItem ;
                                     owl:minCardinality "1"^^xsd:nonNegativeInteger
                                     ] ,
                                     [ rdf:type owl:Restriction ;
                                     owl:onProperty bibrm:price ;
                                     owl:cardinality "1"^^xsd:nonNegativeInteger
                                     ] ,
                                     [ rdf:type owl:Restriction ;
                                     owl:onProperty bibrm:availableAt ;
                                     owl:minCardinality "1"^^xsd:nonNegativeInteger
                                     ] .

bibrm:ContactRole rdf:type      rdfs:Class ;
                  rdfs:label    "Contact Role"@en , "Kontaktart"@de ;
                  rdfs:comment  "A contact role can be used to categorize contacts e.g. customer support, technical support, public relations"@en ,
                                "Eine Kontaktart dient der Einordnung von Kontakten in bestimmte Kategorien bzw. Rollen (z.B. Kundenservice, technischer Support/Service, Marketing usw.)"@de .

########################################
########### ObjectProperties ###########
########################################


bibrm:availableAt rdf:type    owl:ObjectProperty, rdf:Property ;
                  rdfs:comment  "Points to an interface that is usable with a license package"@en ;
                  rdfs:comment  "Ein Hinweis über welches Portal/Interface die Inhalte eines Paktes betrachtet werden können."@de ;
                  rdfs:label  "available at"@en ;
                  rdfs:label  "verfügbar bei"@de ;
                  rdfs:isDefinedBy <> ;
                  rdfs:domain bibrm:LicensePackage ;
                  rdfs:range  bibrm:Interface .

bibrm:hasItem rdf:type    owl:ObjectProperty, rdf:Property ;
              rdfs:comment "Links to items that are part of a license package or a licnense contract"@en ;
              rdfs:comment "Verknüpft Dinge, die Teil eines Lizenzpakets oder eines Lizenzvertrags sind"@de ;
              rdfs:label  "has item"@en ;
              rdfs:label  "besitzt"@de ;
              rdfs:isDefinedBy <> .


bibrm:hasPISSN  rdf:type    owl:ObjectProperty, rdf:Property ;
                rdfs:label  "has P-ISSN"@en ;
                rdfs:label  "hat die P-ISSN"@de ;
                rdfs:isDefinedBy <> ;
                rdfs:domain bibrm:Journal .

bibrm:hasEISSN  rdf:type    owl:ObjectProperty, rdf:Property ;
                rdfs:label  "has E-ISSN"@en ;
                rdfs:label  "hat die E-ISSN"@de ;
                rdfs:isDefinedBy <> ;
                rdfs:domain bibrm:Journal .
                
bibrm:licensor  rdf:type        owl:ObjectProperty, rdf:Property ;
                rdfs:label      "licensor"@en ;
                rdfs:label      "Lizenzgeber"@de ;
                rdfs:comment    "The party of a contract offering the lawfull object/license"@en ;
                rdfs:comment    "Die Vertragspartei, die eine Lizenz zur Verfügung stellt"@de ;
                rdfs:isDefinedBy <> ;
                rdfs:domain     bibrm:LicenseContract ;
                rdfs:range      bibrm:LicensingAgent .

bibrm:licensee  rdf:type        owl:ObjectProperty, rdf:Property ;
                rdfs:label      "licensee"@en ;
                rdfs:label      "Lizenznehmer"@de ;
                rdfs:comment    "The party of a contract receiving the lawfull object/license"@en ;
                rdfs:comment    "Die Vertragspartei, die eine Lizenz erhält"@de ;
                rdfs:isDefinedBy <> ;
                rdfs:domain     bibrm:LicenseContract .

bibrm:usagedatasetupstatus  a            rdf:Property ;
                            rdfs:label   "Usage Data Setup Status" ;
                            rdfs:comment "The StatususagedatasetupstatusThes of the library's arrangement to receive usage data for the product" .

bibrm:usagestatsaddressee   a            rdf:Property ;
                            rdfs:label   "Usage Statistics Addressee" ;
                            rdfs:comment "The local person to whom usagee statistics are sent" .

bibrm:usagestatsavail   a            rdf:Property ;
                        rdfs:label   "Usage Statistics Availability Indicator" ;
                        rdfs:comment "The availability of usage statistics for the product" .

bibrm:usagestatsdelivery    a            rdf:Property ;
                            rdfs:label   "Usage Statisticsstics Delivery Method" ;
                            rdfs:comment "The manner in which usage StatususagedatasetupstatusThesistics are made available" .

bibrm:usagestatsformat  a            rdf:Property ;
                        rdfs:label   "Usage Statistics Format" ;
                        rdfs:comment "The bibrmformat(s) in which usage statistics are made available" .

bibrm:usagestatsfrequency   a            rdf:Property ;
                            rdfs:label   "Usage Statistics Frequency" ;
                            rdfs:comment "The frequency with which usage statistics are made available" .

bibrm:usagestatslocallystored   a            rdf:Property ;
                                rdfs:label   "Information about and/or links to locally-stored usage data" ;
                                rdfs:comment "Usage Statistics Locally Stored" .

bibrm:usagestatsnote    a            rdf:Property ;
                        rdfs:label   "Usage DatatypesStatistics Note" ;
                        rdfs:comment "Additional information regarding usage shortnametatistics" .

bibrm:usagestatsonlinelocation  a            rdf:Property ;
                                rdfs:label   "Usage Statistics Online Location" ;
                                rdfs:comment "The online location at which usage statistics can be accessed" .

bibrm:usagestatspassword    a            rdf:Property ;
                            rdfs:label   "Usage Statistics Password" ;
                            rdfs:comment "The password used for online access to bibrmthe usage statistics management site or dataset" .

bibrm:usagestatsuserid  a            rdf:Property ;
                        rdfs:label   "Usage Statistics User Identifier" ;
                        rdfs:comment "The identifier used for online access to the usage statisticstics file" .

bibrm:counterreporttype a            rdf:Property ;
                        rdfs:label   "COUNTER Report Type" ;
                        rdfs:comment "JR1 etc., s. Dokumentation (multivalue)" .

#################################
########### Datatypes ###########
#################################

bibrm:licenseEndDate   rdf:type    owl:DatatypeProperty, rdf:Property ;
                       rdfs:label  "license end date"@en ;
                       rdfs:label  "Vertragsende"@de ;
                       rdfs:comment "The date on which a license agreement terminates"@en ; 
                       rdfs:comment "Das Datum, an welchem ein Lizenzvertrag endet"@en ; 
                       rdfs:isDefinedBy <> ;
                       rdfs:domain bibrm:LicenseContract ;
                       rdfs:range  xsd:date .

bibrm:field    rdf:type     owl:DatatypeProperty, rdf:Property ;
               rdfs:label   "field"@en ;
               rdfs:label   "Fachgebiet"@de ;
               rdfs:comment "The field predicate can be used to classify bibliographic items"@en ;
               rdfs:comment "Das Prädikat ermgölicht die Angabe von Fachgebieten"@de ;
               rdfs:isDefinedBy <> ;
               rdfs:domain  bibrm:BibItem .

bibrm:name   rdf:type     owl:DatatypeProperty, rdf:Property ;
             rdfs:label   "name"@en ;
             rdfs:label   "Name"@de ;
             rdfs:isDefinedBy <> ;
             rdfs:subPropertyOf  foaf:name .

bibrm:shortname  rdf:type            owl:DatatypeProperty, rdf:Property ;
                 rdfs:label   "shortname"@en ;
                 rdfs:label   "Kurzname"@de ;
                 rdfs:isDefinedBy <> ;
                 rdfs:subPropertyOf  foaf:name .

bibrm:price   rdf:type    owl:DatatypeProperty, rdf:Property ;
            rdfs:label  "price"@en ;
            rdfs:label  "Preis"@de ;
            rdfs:comment    "The price a bibliographic resource costs the library to offer that item to their users"@en ;
            rdfs:comment    "Der Anschaffungs-/Nutzungspreis, den die Bibliothek für eine Bibliographische Ressource bezahlt"@de ;
            rdfs:isDefinedBy <> ;
            rdfs:domain bibrm:BibItem ;
            rdfs:range  xsd:double .

bibrm:publisher  rdf:type    owl:DatatypeProperty, rdf:Property ;
               rdfs:label  "publisher"@en ;
               rdfs:label  "Verlag"@de ;
               rdfs:comment    "The organization which owns the license for a bibliographic resource"@en ;
               rdfs:comment    "Die Institution, die das Recht an einer Bibliographischen Ressource besitzt"@de ;
               rdfs:isDefinedBy <> ;
               rdfs:subPropertyOf  dc:publisher .

bibrm:licenseStartDate   rdf:type    owl:DatatypeProperty, rdf:Property ;
                rdfs:label  "license start date"@en ;
                rdfs:label  "Vertragsbeginn"@de ;
                rdfs:comment "The date on which a license agreement comes into effect"@en ; 
                rdfs:comment "Das Datum, an welchem ein Lizenzvertrag in Kraft tritt"@en ; 
                rdfs:isDefinedBy <> ;
                rdfs:domain bibrm:LicenseContract ;
                rdfs:range  xsd:date .

bibrm:licenseEndDate   rdf:type    owl:DatatypeProperty, rdf:Property ;
                rdfs:label  "license end date"@en ;
                rdfs:label  "Vertragsende"@de ;
                rdfs:comment "The date on which a license agreement loses it's effect"@en ; 
                rdfs:comment "Das Datum, an welchem die Gültigkeit eines Lizenzvertrags endet"@en ; 
                rdfs:isDefinedBy <> ;
                rdfs:domain bibrm:LicenseContract ;
                rdfs:range  xsd:date .

#################################
########### Instances ###########
#################################

bibrm:General         rdf:type  bibrm:ContactRole ;
                      rdfs:label "General information"@en;
                      rdfs:label "Allgemeine Informationen"@de ;
                      rdfs:comment "A Person who acts as contact for general questions"@en;
                      rdfs:comment "Eine Person die als Ansprechpartner für allgemeine Fragen auftritt"@de .
                      
bibrm:CustomerSupport rdf:type  bibrm:ContactRole ;
                      rdfs:label "Customer Support"@en;
                      rdfs:label "Kundenbetreuung"@de ;
                      rdfs:comment "A Person who acts as contact for customer concerns"@en;
                      rdfs:comment "Eine Person die als Ansprechpartner für Anliegen von Kunden auftritt"@de .
                      
bibrm:TechnicalSupport rdf:type  bibrm:ContactRole ;
                      rdfs:label "Technical Support"@en;
                      rdfs:label "Technische Probleme"@de ;
                      rdfs:comment "A Person who acts as contact for technical questions"@en;
                      rdfs:comment "Eine Person die als Ansprechpartner für technische Probleme auftritt"@de .

bibrm:PublicRelations rdf:type  bibrm:ContactRole ;
                      rdfs:label "Public Relations"@en;
                      rdfs:label "Öffentlichkeitsarbeit"@de ;
                      rdfs:comment "A Person who acts as contact for public relations"@en;
                      rdfs:comment "Eine Person die als Ansprechpartner für Öffentlichkeitsarbeit auftritt"@de .

bibrm:Sales           rdf:type  bibrm:ContactRole ;
                      rdfs:label "Sales"@en;
                      rdfs:label "Verkauf"@de ;
                      rdfs:comment "A Person who acts as contact for sale concerns"@en;
                      rdfs:comment "Eine Person die als Ansprechpartner für den Verkauf auftritt"@de .
